\documentclass{article}

\begin{document}
    

$$
b_{n_{left}} = \left\{
        \begin{array}{ll}
            b_{n_{right}} - 1 & \quad b_{z_{left}} \geq 0 \\
            b_{n_{right}} + b_{z_{left}} - 1 & \quad b_{z_{left}} < 0
        \end{array}
    \right.


    b_{z_{left}} = \left\{
        \begin{array}{ll}
            b_{z_{right}} - b_{n_{right}} - 1 & \quad b_{n_{right}} \geq 0 \\
            b_{z_{right}} - 1 & \quad b_{n_{right}} < 0
        \end{array}
    \right.
$$

\end{document}